theories/lang/cpp/logic/expr.v
@@ -736,19 +736,25 @@ Module Type Expr.
         http://www.open-std.org/jtc1/sc22/wg21/docs/papers/2016/p0145r3.pdf
      *)
 
-    (* Due to our non-standard calling convention (the fact that [fspec]
+    (* TODO fix this comment.
+       Due to our non-standard calling convention (the fact that [fspec]
        "returns" a [val] rather than a [ptr]), there is some processing
        that we must do to the result. We consolidate these definitions here
        because they are shared between function and member function calls.
      *)
-    Definition xval_receive (res : val) (Q : ptr -> mpred) : mpred :=
-      Exists p, [| res = Vptr p |] ** Q p.
-    Definition lval_receive (res : val) (Q : ptr -> mpred) : mpred :=
-      Exists p, [| res = Vptr p |] ** Q p.
-    Definition operand_receive (ty : type) (res : val) (Q : val -> (FreeTemps -> FreeTemps) -> mpred) : mpred :=
-      Q res (fun x => x).
-    Definition init_receive (ty : type) (addr : ptr) (res : val) (Q : FreeTemp -> mpred) : mpred :=
-      Exists p, [| res = Vptr p |] ** ([| p = addr |] -* Q (FreeTemps.delete ty addr)).
+    Definition xval_receive (ty : type) (res : ptr) (Q : ptr -> mpred) : mpred :=
+      Exists p, res |-> primR ty 1 (Vref p) ** Q p.
+    Definition lval_receive (ty : type) (res : ptr) (Q : ptr -> mpred) : mpred :=
+      Exists p, res |-> primR ty 1 (Vref p) ** Q p.
+    Definition operand_receive (ty : type) (res : ptr) (Q : val -> (FreeTemps -> FreeTemps) -> mpred) : mpred :=
+      match ty with
+      | Tvoid =>
+        [| res = invalid_ptr |] ** Q Vvoid (fun x => x)
+      | _ =>
+        Exists v, res |-> primR ty 1 v ** Q v (fun x => x)
+      end.
+    Definition init_receive (ty : type) (addr : ptr) (res : ptr) (Q : FreeTemp -> mpred) : mpred :=
+      ([| addr = res |] -* Q (FreeTemps.delete ty addr)).
 
     (** [wp_call pfty f es Q] calls [f] taking the arguments from the
         evaluations of [es] and then acts like [Q].
@@ -762,7 +768,7 @@ Module Type Expr.
              qualifiers is addressed through the use of [normalize_type]
              below.
      *)
-    Definition wp_call (pfty : type) (f : val) (es : list Expr) (Q : val -> FreeTemps -> epred) : mpred :=
+    Definition wp_call (pfty : type) (f : val) (es : list Expr) (Q : ptr -> FreeTemps -> epred) : mpred :=
       match unptr pfty with
       | Some fty =>
         let fty := normalize_type fty in
@@ -777,12 +783,12 @@ Module Type Expr.
 
     Axiom wp_lval_call : forall f (es : list Expr) Q (ty : type),
         wp_operand f (fun fn free_f => wp_call (type_of f) fn es $ fun res free_args =>
-           Reduce (lval_receive res $ fun v => Q v (free_args >*> free_f)))
+           Reduce (lval_receive (Tref ty) res $ fun v => Q v (free_args >*> free_f)))
         |-- wp_lval (Ecall f es ty) Q.
 
     Axiom wp_xval_call : forall f (es : list Expr) Q (ty : type),
         wp_operand f (fun fn free_f => wp_call (type_of f) fn es $ fun res free_args =>
-           Reduce (xval_receive res $ fun v => Q v (free_args >*> free_f)))
+           Reduce (xval_receive (Trv_ref ty) res $ fun v => Q v (free_args >*> free_f)))
         |-- wp_xval (Ecall f es ty) Q.
 
     Axiom wp_operand_call : forall ty f es Q,
@@ -797,7 +803,6 @@ Module Type Expr.
       |-- wp_init addr (Ecall f es ty) Q.
 
     (** * Member calls *)
-
     Definition member_arg_types (fty : type) : option (list type) :=
       match fty with
       | @Tfunction _ _ (_ :: args) => Some args
@@ -805,23 +810,23 @@ Module Type Expr.
       end.
 
     Definition wp_mcall (f : val) (this : ptr) (this_type : type) (fty : type) (es : list Expr)
-               (Q : val -> FreeTemps -> epred) : mpred :=
+               (Q : ptr -> FreeTemps -> epred) : mpred :=
       let fty := normalize_type fty in
       Exists fp, [| f = Vptr fp|] **
       match arg_types fty with
       | Some targs =>
-        wp_args targs es $ fun vs free => |> mspec this_type fty fp (Vptr this :: vs) (fun v => Q v free)
+        wp_args targs es $ fun vs free => |> mspec this_type fty fp (this :: vs) (fun v => Q v free)
       | _ => False
       end.
 
     Axiom wp_lval_member_call : forall ty fty f vc obj es Q,
         wp_glval vc obj (fun this free_this => wp_mcall (Vptr $ _global f) this (type_of obj) fty es $ fun res free_args =>
-           lval_receive res $ fun v => Q v (free_args >*> free_this))
+           lval_receive ty res $ fun v => Q v (free_args >*> free_this))
         |-- wp_lval (Emember_call (inl (f, Direct, fty)) vc obj es ty) Q.
 
     Axiom wp_xval_member_call : forall ty fty f vc obj es Q,
         wp_glval vc obj (fun this free_this => wp_mcall (Vptr $ _global f) this (type_of obj) fty es $ fun res free_args =>
-           xval_receive res $ fun v => Q v (free_args >*> free_this))
+           xval_receive ty res $ fun v => Q v (free_args >*> free_this))
         |-- wp_xval (Emember_call (inl (f, Direct, fty)) vc obj es ty) Q.
 
     Axiom wp_operand_member_call : forall ty fty f vc obj es Q,
@@ -845,7 +850,7 @@ Module Type Expr.
         the called method is a [const] method. This matches the construction of [SMethod].
      *)
     Definition wp_virtual_call (f : obj_name) (this : ptr) (this_type : type) (fty : type) (es : list Expr)
-               (Q : val -> FreeTemps -> epred) : mpred :=
+               (Q : ptr -> FreeTemps -> epred) : mpred :=
       match decompose_type this_type with
       | (tq, Tnamed cls) =>
         resolve_virtual (σ:=resolve) this cls f (fun fimpl_addr impl_class thisp =>
@@ -855,12 +860,12 @@ Module Type Expr.
 
     Axiom wp_xval_virtual_call : forall ty fty f vc obj es Q,
         wp_glval vc obj (fun this free_this => wp_virtual_call f this (type_of obj) fty es $ fun res free_args =>
-                   xval_receive res $ fun v => Q v (free_args >*> free_this))
+                   xval_receive ty res $ fun v => Q v (free_args >*> free_this))
       |-- wp_xval (Emember_call (inl (f, Virtual, fty)) vc obj es ty) Q.
 
     Axiom wp_lval_virtual_call : forall ty fty f vc obj es Q,
         wp_glval vc obj (fun this free_this => wp_virtual_call f this (type_of obj) fty es $ fun res free_args =>
-                   lval_receive res $ fun v => Q v (free_args >*> free_this))
+                   lval_receive ty res $ fun v => Q v (free_args >*> free_this))
       |-- wp_lval (Emember_call (inl (f, Virtual, fty)) vc obj es ty) Q.
 
     Axiom wp_operand_virtual_call : forall ty fty f vc obj es Q,
@@ -985,9 +990,10 @@ Module Type Expr.
            match resolve.(genv_tu) !! cnd with
            | Some cv =>
              addr |-> tblockR (Tnamed cls) 1 -*
-             (* ^^ Our semantics currently has constructors take ownership of a [tblockR] *)
+             (* ^^ The semantics currently has constructors take ownership of a [tblockR] *)
              wp_mcall (Vptr $ _global cnd) addr (Tnamed cls) (type_of_value cv) es (fun v free =>
-                [| v = Vundef |] ** Q (FreeTemps.delete (Tnamed cls) addr) free)
+               (* in the semantics, constructors return [void] *)
+               [| v = invalid_ptr |] ** Q (FreeTemps.delete (Tnamed cls) addr) free)
            | _ => False
            end
       |-- wp_init addr (Econstructor cnd es (Tnamed cls)) Q.
